work on stack_allocProof

compiler/backend/stack_allocScript.sml
@@ -36,7 +36,7 @@ val comp_def = Define `
           | SOME (p2,k1,k2) =>
               let (q2,m) = comp n m p2 in
                 (Call (SOME (q1,lr,l1,l2)) dest (SOME (q2,k1,k2)),m))
-    | Alloc n => (Call (SOME (Skip,0,n,m)) (INL 10) NONE,m+1)
+    | Alloc k => (Call (SOME (Skip,0,n,m)) (INL 10) NONE,m+1)
     | _ => (p,m) `
 
 val prog_comp_def = Define `
