compiler/backend/proofs/stack_allocProofScript.sml
@@ -1,0 +1,204 @@
+open preamble
+     stack_allocTheory
+     stackSemTheory
+     stackPropsTheory
+
+val _ = new_theory"stack_allocProof";
+
+val good_syntax_def = Define `
+  (good_syntax (Alloc v) <=> (v = 1)) /\
+  (good_syntax ((Seq p1 p2):'a stackLang$prog) <=>
+     good_syntax p1 /\ good_syntax p2) /\
+  (good_syntax ((If c r ri p1 p2):'a stackLang$prog) <=>
+     good_syntax p1 /\ good_syntax p2) /\
+  (good_syntax (Call x1 _ x2) <=>
+     (case x1 of | SOME (y,r,_,_) => good_syntax y | NONE => T) /\
+     (case x2 of SOME (y,_,_) => good_syntax y | NONE => T)) /\
+  (good_syntax _ <=> T)`
+
+val get_var_imm_case = prove(
+  ``get_var_imm ri s =
+    case ri of
+    | Reg n => get_var n s
+    | Imm w => SOME (Word w)``,
+  Cases_on `ri` \\ fs [get_var_imm_def]);
+
+val prog_comp_lemma = prove(
+  ``prog_comp = \(n,p). (n,FST (comp n (next_lab p) p))``,
+  fs [FUN_EQ_THM,FORALL_PROD,prog_comp_def]);
+
+val ALOOKUP_MAP_ALT = prove(
+  ``(!x n y m. (f (x,n) = (y,m)) ==> x = y) ==>
+    (ALOOKUP (MAP f xs) n =
+     case ALOOKUP xs n of
+     | NONE => NONE
+     | SOME x => SOME (SND (f(n,x))))``,
+  Induct_on `xs` \\ fs [] \\ Cases \\ fs [ALOOKUP_def,FORALL_PROD]
+  \\ rw [] \\ fs [] \\ Cases_on `f (n,r)` \\ fs [ALOOKUP_def] \\ res_tac \\ fs []
+  \\ rw [] \\ fs [] \\ Cases_on `f (q,r)` \\ fs [ALOOKUP_def] \\ res_tac \\ fs [])
+
+val lookup_IMP_lookup_compile = prove(
+  ``lookup dest s.code = SOME x /\ 30 <= dest ==>
+    ?m1 n1. lookup dest (fromAList (compile c (toAList s.code))) =
+            SOME (FST (comp m1 n1 x))``,
+  fs [lookup_fromAList,compile_def] \\ rw [ALOOKUP_APPEND]
+  \\ `ALOOKUP (stubs c) dest = NONE` by
+    (fs [stubs_def] \\ rw [] \\ fs [] \\ decide_tac) \\ fs []
+  \\ fs [prog_comp_lemma] \\ fs [ALOOKUP_MAP_ALT,ALOOKUP_toAList]
+  \\ metis_tac []);
+
+val alloc_correct = prove(
+  ``alloc w s = (r,t) /\ r <> SOME Error /\
+    FLOOKUP s.regs 1 = SOME (Word w) ==>
+    ?ck. evaluate
+          (Call (SOME (Skip,0,n',m)) (INL 10) NONE,
+           s with
+           <|use_alloc := F; clock := s.clock + ck;
+             code := fromAList (compile c (toAList s.code))|>) =
+         (r,
+          t with
+           <|use_alloc := F; code := fromAList (compile c (toAList s.code))|>)``,
+  cheat (* correctness of stubs *));
+
+val find_code_IMP_lookup = prove(
+  ``find_code dest regs (s:'a num_map) = SOME x ==>
+    ?k. lookup k s = SOME x /\
+        (find_code dest regs = ((lookup k):'a num_map -> 'a option))``,
+  Cases_on `dest` \\ fs [find_code_def,FUN_EQ_THM]
+  \\ every_case_tac \\ fs [] \\ metis_tac []);
+
+val comp_correct = prove(
+  ``!p s r t m n c.
+      evaluate (p,s) = (r,t) /\ r <> SOME Error /\ good_syntax p /\
+      (!k prog. lookup k s.code = SOME prog ==> 30 <= k /\ good_syntax prog) ==>
+      ?ck.
+        evaluate (FST (comp n m p),
+           s with <| clock := s.clock + ck;
+                     code := fromAList (stack_alloc$compile c (toAList s.code));
+                     use_alloc := F |>) =
+          (r, t with
+              <| code := fromAList (stack_alloc$compile c (toAList s.code));
+                 use_alloc := F |>)``,
+  recInduct evaluate_ind \\ rpt strip_tac
+  THEN1 (* Skip *)
+   (fs [Once comp_def,evaluate_def] \\ rw [] \\ fs [state_component_equality])
+  THEN1 (* Halt *)
+   (fs [Once comp_def,evaluate_def,get_var_def]
+    \\ CASE_TAC \\ fs [] \\ rw [] \\ fs [state_component_equality])
+  THEN1 (* Alloc *)
+   (fs [evaluate_def,get_var_def]
+    \\ fs [Once comp_def,get_var_def]
+    \\ every_case_tac \\ fs [good_syntax_def] \\ rw []
+    \\ drule alloc_correct \\ fs [])
+  THEN1 (* Inst *)
+   (fs [Once comp_def] \\ fs [evaluate_def,inst_def]
+    \\ CASE_TAC \\ fs [] \\ rw []
+    \\ fs [assign_def,word_exp_def,set_var_def,mem_load_def,
+         get_var_def,mem_store_def]
+    \\ rw [] \\ fs [] \\ fs [state_component_equality]
+    \\ every_case_tac \\ fs [markerTheory.Abbrev_def,LET_DEF,word_exp_def]
+    \\ fs [state_component_equality] \\ rw [])
+  THEN1 (* Get *)
+   (fs [Once comp_def,evaluate_def,get_var_def]
+    \\ every_case_tac \\ fs [] \\ rw [] \\ fs [set_var_def]
+    \\ fs [state_component_equality])
+  THEN1 (* Set *)
+   (fs [Once comp_def,evaluate_def,get_var_def,set_store_def]
+    \\ every_case_tac \\ fs [] \\ rw [] \\ fs [set_var_def]
+    \\ fs [state_component_equality])
+  THEN1 (* Tick *)
+   (qexists_tac `0` \\ fs [Once comp_def,evaluate_def,dec_clock_def]
+    \\ every_case_tac \\ fs [] \\ rw [] \\ fs [set_var_def]
+    \\ fs [state_component_equality,empty_env_def])
+  THEN1 (* Seq *)
+   (simp [Once comp_def,dec_clock_def] \\ fs [evaluate_def]
+    \\ split_pair_tac \\ fs [LET_DEF]
+    \\ split_pair_tac \\ fs [LET_DEF]
+    \\ split_pair_tac \\ fs [LET_DEF]
+    \\ fs [good_syntax_def,evaluate_def]
+    \\ first_x_assum (qspecl_then[`m`,`n`,`c`]mp_tac)
+    \\ match_mp_tac IMP_IMP \\ conj_tac
+    THEN1 (CCONTR_TAC \\ fs [] \\ fs [] \\ res_tac)
+    \\ strip_tac \\ rfs[]
+    \\ reverse (Cases_on `res`) \\ fs []
+    THEN1 (qexists_tac `ck` \\ fs [AC ADD_COMM ADD_ASSOC,LET_DEF] \\ rw [])
+    \\ first_x_assum (qspecl_then[`m'`,`n`,`c`]mp_tac)
+    \\ match_mp_tac IMP_IMP \\ conj_tac
+    THEN1 (rw [] \\ imp_res_tac evaluate_consts \\ fs [] \\ res_tac \\ fs [])
+    \\ strip_tac \\ pop_assum mp_tac
+    \\ drule (GEN_ALL evaluate_add_clock) \\ simp []
+    \\ disch_then (qspec_then `ck'`assume_tac) \\ strip_tac
+    \\ qexists_tac `ck + ck'` \\ fs [AC ADD_COMM ADD_ASSOC]
+    \\ imp_res_tac evaluate_consts \\ fs [])
+  THEN1 (* Return *)
+   (qexists_tac `0` \\ fs [Once comp_def,evaluate_def,get_var_def]
+    \\ every_case_tac \\ fs [] \\ rw [] \\ fs [get_var_def]
+    \\ fs [state_component_equality,empty_env_def])
+  THEN1 (* Raise *)
+   (qexists_tac `0` \\ fs [Once comp_def,evaluate_def,get_var_def]
+    \\ every_case_tac \\ fs [] \\ rw [] \\ fs [get_var_def]
+    \\ fs [state_component_equality,empty_env_def])
+  THEN1 (* If *)
+   (simp [Once comp_def] \\ fs [evaluate_def,get_var_def]
+    \\ split_pair_tac \\ fs [] \\ split_pair_tac \\ fs []
+    \\ every_case_tac \\ fs []
+    \\ fs [evaluate_def,get_var_def,get_var_imm_case,good_syntax_def]
+    \\ rfs []
+    THENL [first_x_assum (qspecl_then[`m`,`n`,`c`]mp_tac),
+           first_x_assum (qspecl_then[`m'`,`n`,`c`]mp_tac)]
+    \\ match_mp_tac IMP_IMP \\ conj_tac
+    \\ TRY (rw [] \\ res_tac \\ fs [] \\ NO_TAC)
+    \\ strip_tac \\ fs [] \\ rfs []
+    \\ qexists_tac `ck` \\ fs [AC ADD_COMM ADD_ASSOC])
+  THEN1 (* JumpLess *)
+   (fs [evaluate_def,get_var_def] \\ simp [Once comp_def]
+    \\ every_case_tac \\ fs [] \\ rw [] \\ fs [good_syntax_def]
+    \\ fs [evaluate_def,get_var_def] \\ fs [find_code_def]
+    \\ fs [state_component_equality,empty_env_def] \\ res_tac
+    \\ imp_res_tac lookup_IMP_lookup_compile
+    \\ pop_assum (qspec_then `c` strip_assume_tac) \\ fs []
+    THEN1 (qexists_tac `0` \\ fs [state_component_equality,empty_env_def])
+    \\ rfs [] \\ fs [PULL_FORALL,dec_clock_def]
+    \\ first_x_assum (qspecl_then[`m1`,`n1`,`c`]mp_tac)
+    \\ match_mp_tac IMP_IMP \\ conj_tac
+    \\ TRY (rw [] \\ res_tac \\ fs [] \\ NO_TAC) \\ strip_tac \\ fs []
+    \\ `ck + s.clock - 1 = ck + (s.clock - 1)` by decide_tac
+    \\ qexists_tac `ck` \\ fs [AC ADD_COMM ADD_ASSOC])
+  THEN1 (* Call *)
+   (fs [evaluate_def] \\ Cases_on `find_code dest s.regs s.code` \\ fs []
+    \\ Cases_on `ret` \\ fs [] THEN1
+     (every_case_tac \\ fs [empty_env_def] \\ rw [] \\ fs []
+      \\ fs [good_syntax_def] \\ simp [Once comp_def,evaluate_def]
+      \\ drule find_code_IMP_lookup \\ fs [] \\ rw [] \\ fs [] \\ fs []
+      \\ res_tac \\ imp_res_tac lookup_IMP_lookup_compile
+      \\ pop_assum (strip_assume_tac o SPEC_ALL) \\ fs []
+      THEN1 (qexists_tac `0` \\ fs [empty_env_def,state_component_equality])
+      THEN1 (qexists_tac `0` \\ fs [empty_env_def,state_component_equality])
+      \\ fs [dec_clock_def]
+      \\ first_x_assum (qspecl_then[`n1`,`m1`,`c`]mp_tac)
+      \\ match_mp_tac IMP_IMP \\ conj_tac
+      \\ TRY (rw [] \\ res_tac \\ fs [] \\ NO_TAC) \\ strip_tac \\ fs []
+      \\ `ck + s.clock - 1 = ck + (s.clock - 1)` by decide_tac
+      \\ qexists_tac `ck` \\ fs [AC ADD_COMM ADD_ASSOC])
+    \\ qmatch_assum_rename_tac `good_syntax (Call (SOME z) dest handler)`
+    \\ PairCases_on `z` \\ fs [] \\ simp [Once comp_def] \\ fs []
+    \\ split_pair_tac \\ fs []
+    \\ cheat (* Call case is full of similar cases *))
+  THEN1 (* FFI *)
+   (qexists_tac `0` \\ fs [Once comp_def,evaluate_def,get_var_def]
+    \\ every_case_tac \\ fs [] \\ rw [] \\ fs [get_var_def]
+    \\ fs [state_component_equality,empty_env_def,LET_DEF])
+  \\ qexists_tac `0` \\ fs [Once comp_def,evaluate_def,get_var_def,set_var_def]
+  \\ every_case_tac \\ fs [] \\ rw [] \\ fs [get_var_def]
+  \\ fs [state_component_equality,empty_env_def,LET_DEF]);
+
+val compile_semantics = store_thm("compile_semantics",
+  ``(!k prog. lookup k s.code = SOME prog ==> 30 < k /\ good_syntax prog) /\
+    semantics start s <> Fail ==>
+    semantics start (s with <|
+                       code := fromAList (stack_alloc$compile c (toAList s.code));
+                       use_alloc := F |>) =
+    semantics start s``,
+  cheat);
+
+val _ = export_theory();
